Clean up `Integer.lean`
- Removed unnecessary check in `instOfNat`
- Removed unnecessary `Int16.` and `Integer.` prefixes
- Put everything into `Int16` or `Integer` namespace
- Changed `Repr` instance to return just the integer literal
- added tests for the `ToExpr` instance

Shenzhen/Integer.lean
@@ -9,7 +9,15 @@ structure Integer where
   n : Int16
   le : n ≤ 999 := by decide
   ge : -999 ≤ n := by decide
-deriving DecidableEq, BEq, Fintype, Repr
+deriving DecidableEq, BEq, Fintype
+
+namespace Integer
+
+instance : Repr Integer where
+  reprPrec x prec := reprPrec x.n prec
+
+instance : ReprAtom Integer :=
+  .mk
 
 instance : ToString Integer :=
   ⟨(toString ·.n)⟩
@@ -20,24 +28,34 @@ instance : Inhabited Integer :=
 instance : Coe Integer Int16 :=
   ⟨(·.n)⟩
 
-def Integer.ofInt (n : Int) (h₁ : n ≤ 999) (h₂ : -999 ≤ n) :=
-  have : Int16.ofInt n ≤ Int16.ofInt 999 ∧ Int16.ofInt (-999) ≤ Int16.ofInt n := by
+open Int16
+
+def ofInt (n : Int) (h₁ : n ≤ 999) (h₂ : -999 ≤ n) :=
+  have : Int16.ofInt n ≤ .ofInt 999 ∧ Int16.ofInt (-999) ≤ .ofInt n := by
     constructor <;> (
       apply (Int16.ofInt_le_iff_le ..).mpr
       all_goals first | trivial | grind only)
-  Integer.mk (Int16.ofInt n) this.left this.right
+  Integer.mk (.ofInt n) this.left this.right
 
-instance instOfNatInteger : OfNat Integer n where
+instance {n} : OfNat Integer n where
   ofNat :=
-    let n' := n.toInt16
-    if h : -999 ≤ n' ∧ n' ≤ 999 then
-      ⟨n', h.right, h.left⟩
-    else panic! "In `instOfNatInteger`: argument is not in [-999, 999]!"
+    if h : n ≤ 999 then
+      have := Nat.lt_of_le_of_lt h (by decide)
+      have h₁ :=
+        @ofNat_le_iff_le n 999 this (by decide)|>.mpr h
+      have h₂ := Int16.le_trans (b := 0) (by decide) <|
+        zero_le_ofNat_of_lt this
+      ⟨Int16.ofNat n, h₁, h₂⟩
+    else panic! "In `instOfNatInteger`: argument is > 999!"
+
+/-- Clamp negative values to `(0 : Nat)`. -/
+@[inline] def clampToNat : Integer → Nat
+| { n, .. } => n.toNatClampNeg
 
 /-- Lift a binary operation on `Int16`s to `Integer`s by clamping the result
 to `[-999, 999]`. -/
 @[inline, specialize]
-private def Integer.liftOp (f : Int16 → Int16 → Int16) : Integer → Integer → Integer
+private def liftOp (f : Int16 → Int16 → Int16) : Integer → Integer → Integer
 | ⟨a, _, _⟩, ⟨b, _, _⟩ => ⟨
   Clamp.clamp (f a b) (-999) 999,
   Clamp.clamp_le_hi (by decide), Clamp.lo_le_clamp (by decide)⟩
@@ -52,7 +70,11 @@ instance : Complement Integer where
   | ⟨0, _, _⟩ => 100
   | _ => 0
 
-theorem Int16.eq_minValue_iff_dvd_toInt {a : Int16} : (a = .minValue ∨ a = 0) ↔ 2^15 ∣ a.toInt := by
+end Integer
+
+namespace Int16
+
+theorem eq_minValue_iff_dvd_toInt {a : Int16} : (a = .minValue ∨ a = 0) ↔ 2^15 ∣ a.toInt := by
   constructor
   · rintro (h|h) <;> (rw [h]; decide)
   · intro ⟨k, hk⟩
@@ -61,10 +83,10 @@ theorem Int16.eq_minValue_iff_dvd_toInt {a : Int16} : (a = .minValue ∨ a = 0) 
       rw [show (2^15: Int) * 1 = 32767 + 1 by decide]
       apply Int.lt_add_one_of_le
       rw [←hk]
-      apply Int16.toInt_le _
+      apply toInt_le
     have hk_ge : k ≥ -1 := by
       refine Int.not_lt.mp fun hn => ?_
-      refine absurd (Int16.le_toInt a) (Int.not_le_of_gt ?_)
+      refine absurd (le_toInt a) (Int.not_le_of_gt ?_)
       rw [hk]
       exact Int.mul_lt_mul_of_pos_left hn (by decide)
 
@@ -72,45 +94,51 @@ theorem Int16.eq_minValue_iff_dvd_toInt {a : Int16} : (a = .minValue ∨ a = 0) 
     | -1 =>
       left
       rwa [show (2^15: Int) * (-1) = (-2^15: Int16).toInt by decide,
-           Int16.toInt_inj
+           toInt_inj
       ] at hk
     | 0 =>
       right
       rwa [show (2^15: Int) * 0 = (0: Int16).toInt by decide,
-           Int16.toInt_inj
+           toInt_inj
       ] at hk
 
-theorem Int16.toInt_neg' {a : Int16} (ha : a ≠ .minValue) : (-a).toInt = -(a.toInt) := by
-  rw [Int16.toInt_neg, Int.neg_bmod]
+theorem toInt_neg' {a : Int16} (ha : a ≠ .minValue) : (-a).toInt = -(a.toInt) := by
+  rw [toInt_neg, Int.neg_bmod]
   simp only [Nat.reducePow, Int.cast_ofNat_Int, toInt_bmod]
   simp only [show (65536: Int) = 2 * 2^15 by decide,
             @Int.mul_dvd_mul_iff_left 2 _ _ (by decide)]
-  simp only [←Int16.eq_minValue_iff_dvd_toInt, ha, false_or]
+  simp only [←eq_minValue_iff_dvd_toInt, ha, false_or]
   split <;> simp_all
 
-theorem Int16.mod_lt_of_pos (a : Int16) {b : Int16} (hb : b > 0) : a % b < b := by
+theorem mod_lt_of_pos (a : Int16) {b : Int16} (hb : b > 0) : a % b < b := by
   rw [lt_iff_toInt_lt, toInt_mod]
   apply Int.tmod_lt_of_pos
   rwa [←toInt_zero, ←lt_iff_toInt_lt]
 
-theorem Int16.lt_mod_of_pos (a : Int16) {b : Int16} (hb : b > 0) : -b < a % b := by
+theorem lt_mod_of_pos (a : Int16) {b : Int16} (hb : b > 0) : -b < a % b := by
   rw [lt_iff_toInt_lt,
-      @Int16.toInt_neg' b (by intro; simp_all),
+      @toInt_neg' b (by intro; simp_all),
       toInt_mod]
   apply Int.lt_tmod_of_pos
   rwa [←toInt_zero, ←lt_iff_toInt_lt]
 
-theorem Int16.neg_le_neg_iff {a b : Int16} (ha : a ≠ .minValue) (hb : b ≠ .minValue) : -a ≤ -b ↔ b ≤ a := by
-  rw [Int16.le_iff_toInt_le, Int16.le_iff_toInt_le]
-  rw [Int16.toInt_neg' ha, Int16.toInt_neg' hb]
+theorem neg_le_neg_iff {a b : Int16} (ha : a ≠ .minValue) (hb : b ≠ .minValue) : -a ≤ -b ↔ b ≤ a := by
+  rw [le_iff_toInt_le, le_iff_toInt_le]
+  rw [toInt_neg' ha, toInt_neg' hb]
   simp
 
+end Int16
+
+namespace Integer
+
+open Int16
+
 /-- `dgt` stands for "digit get." It preserves sign. -/
-def Integer.dgt (acc target : Integer) : Integer :=
+def dgt (acc target : Integer) : Integer :=
   have h₁ {n : Int16} : n % 10 ≤ 999 :=
-    Int16.le_of_lt (Int16.lt_of_lt_of_le (Int16.mod_lt_of_pos n (by decide)) (by decide))
+    Int16.le_of_lt (Int16.lt_of_lt_of_le (mod_lt_of_pos n (by decide)) (by decide))
   have h₂ {n : Int16} : -999 ≤ n % 10 :=
-    Int16.le_of_lt (Int16.lt_of_le_of_lt (by decide) (Int16.lt_mod_of_pos n (by decide)))
+    Int16.le_of_lt (Int16.lt_of_le_of_lt (by decide) (lt_mod_of_pos n (by decide)))
 
   match target with
   | ⟨0, _, _⟩ => ⟨acc.n % 10, h₁, h₂⟩
@@ -119,7 +147,7 @@ def Integer.dgt (acc target : Integer) : Integer :=
   | _ => 0
 
 /-- `dst` stands for "digit set" -/
-def Integer.dst (_acc _target _new : Integer) : Integer :=
+def dst (_acc _target _new : Integer) : Integer :=
   -- In case `new` is outside [-9, 9]
   -- let newDigit := new.n % 10 -- with the same sign as `new`
   panic! "`dst` is unimplemented!" -- TODO
@@ -128,16 +156,16 @@ def Integer.dst (_acc _target _new : Integer) : Integer :=
 instance : Neg Integer where
   neg
   | ⟨n, le, ge⟩ =>
-    have : n ≠ Int16.minValue := by
+    have : n ≠ minValue := by
       intro hn
       rw [hn] at ge
       contradiction
     {
       n := -n,
-      le := show -n ≤ - -999 from
-        (Int16.neg_le_neg_iff this (by decide)).mpr ge,
+      le := show -n ≤ - -999 from -- this hint speeds up elaboration significantly
+        (neg_le_neg_iff this (by decide)).mpr ge,
       ge :=
-        (Int16.neg_le_neg_iff (by decide) this).mpr le
+        (neg_le_neg_iff (by decide) this).mpr le
     }
 
 instance : LT Integer :=
@@ -165,14 +193,36 @@ where
       (mkApp4 (mkConst ``LE.le [0]) (mkConst ``Int16) (mkConst ``instLEInt16) a b)
       (mkApp2 (mkConst ``Int16.decLe) a b)
 
--- elab "test " sign:("-" noWs)? x:num : term =>
---   let n : Int := (if sign.isSome then -1 else 1) * x.getNat
---   if h : n ≤ 999 ∧ -999 ≤ n then
---     return Lean.ToExpr.toExpr (Integer.ofInt n h.left h.right)
---   else throwError "invalid literal provided"
+elab "test_Integer.instToExpr" sign:("-" noWs)? x:num : term =>
+  let n : Int := (if sign.isSome then -1 else 1) * x.getNat
+  if h : n ≤ 999 ∧ -999 ≤ n then
+    return Lean.ToExpr.toExpr (Integer.ofInt n h.left h.right)
+  else throwError "invalid literal provided"
 
--- #check test -3
+/-- error: invalid literal provided -/
+#guard_msgs in
+#check test_Integer.instToExpr -1103
 
-/-- Clamp negative values to `(0 : Nat)`. -/
-@[inline] def Integer.clampToNat : Integer → Nat
-| { n, .. } => n.toNatClampNeg
+/-- info: { n := -999, le := ⋯, ge := ⋯ } : Integer -/
+#guard_msgs in
+#check test_Integer.instToExpr -999
+
+/-- info: { n := -15, le := ⋯, ge := ⋯ } : Integer -/
+#guard_msgs in
+#check test_Integer.instToExpr -15
+
+/-- info: { n := 0, le := ⋯, ge := ⋯ } : Integer -/
+#guard_msgs in
+#check test_Integer.instToExpr 0
+
+/-- info: { n := 37, le := ⋯, ge := ⋯ } : Integer -/
+#guard_msgs in
+#check test_Integer.instToExpr 37
+
+/-- info: { n := 999, le := ⋯, ge := ⋯ } : Integer -/
+#guard_msgs in
+#check test_Integer.instToExpr 999
+
+/-- error: invalid literal provided -/
+#guard_msgs in
+#check test_Integer.instToExpr 8314
